LeanMathLogicExploration/RelationalAlgebra/Relation.lean
@@ -4,4 +4,5 @@ import  «LeanMathLogicExploration».RelationalAlgebra.Core
 import  «LeanMathLogicExploration».RelationalAlgebra.Order
 import  «LeanMathLogicExploration».RelationalAlgebra.Eq
 import  «LeanMathLogicExploration».RelationalAlgebra.Union
--- import  «LeanMathLogicExploration».RelationalAlgebra.Intersection
+import  «LeanMathLogicExploration».RelationalAlgebra.Intersection
+import  «LeanMathLogicExploration».RelationalAlgebra.Logic
