LeanMathLogicExploration/RelationalPrograms.lean
@@ -1,4 +1,0 @@
--- In this file I'm writing compositional formulas for common manipulations of relations.
-
-
--- A selection relation is a subre
